rustfrontend/BorrowCheckSafe.v
@@ -1,0 +1,40 @@
+Require Import Coqlib.
+Require Import Errors.
+Require Import Values.
+Require Import AST Errors.
+Require Import Memory.
+Require Import Events.
+Require Import Globalenvs.
+Require Import Smallstep SmallstepLinkingSafe.
+Require Import LanguageInterface Invariant.
+Require Import Rusttypes.
+Require Import RustIR BorrowCheckPolonius.
+
+Section BORROWCK.
+
+Variable p tp: program.
+Variable se: Genv.symtbl.
+Hypothesis BORCHK: borrow_check_program p = OK tp.
+Hypothesis VALIDSE: Genv.valid_for (erase_program p) se.
+
+Let L1 := semantics p se.
+Let L2 := semantics tp se.
+
+
+Lemma sound_state_safe: forall s,
+    partial_safe L1 s ->
+    safe L2 s.
+Admitted.
+
+End BORROWCK.
+
+
+Lemma borrow_check_safe: forall p tp,
+    borrow_check_program p = OK tp ->
+    module_safe (semantics p) wt_c wt_c partial_safe ->
+    module_safe (semantics tp) wt_c wt_c safe.
+Proof.
+  intros p tp BORCHK MSAFE.
+  red. intros w se VALIDSE SYMBINV.
+Admitted.
+    
